cedar-lean/Cedar/Partial/Value.lean
@@ -23,18 +23,54 @@ This file defines Cedar partial values.
 
 namespace Cedar.Partial
 
+open Cedar.Data
+
 inductive Value where
   | value (v : Spec.Value)
   | residual (r : Partial.Expr)
 
 deriving instance Repr, DecidableEq, Inhabited for Value
 
-def Value.asPartialExpr (v : Partial.Value) : Partial.Expr :=
-  match v with
+def Value.asPartialExpr : Partial.Value → Partial.Expr
   | .value v    => v.asPartialExpr
   | .residual r => r
 
 instance : Coe Spec.Value Partial.Value where
   coe := Partial.Value.value
+
+/--
+  Given a map of unknown-name to value, substitute all unknowns with the
+  corresponding values, producing a new `Partial.Expr`.
+  It's fine for some unknowns to not be in `subsmap`, in which case the returned
+  `Partial.Expr` will still contain some unknowns.
+-/
+-- NB: this function can't live in Partial/Expr.lean because it needs Partial.Value, and
+-- Partial/Expr.lean can't import Partial/Value.lean, cyclic dependency
+def Expr.subst (subsmap : Map Unknown Partial.Value) : Partial.Expr → Partial.Expr
+  | .lit p => .lit p -- no unknowns, nothing to substitute
+  | .var v => .var v -- no unknowns, nothing to substitute
+  | .ite x₁ x₂ x₃ => .ite (x₁.subst subsmap) (x₂.subst subsmap) (x₃.subst subsmap)
+  | .and x₁ x₂ => .and (x₁.subst subsmap) (x₂.subst subsmap)
+  | .or x₁ x₂ => .or (x₁.subst subsmap) (x₂.subst subsmap)
+  | .unaryApp op x₁ => .unaryApp op (x₁.subst subsmap)
+  | .binaryApp op x₁ x₂ => .binaryApp op (x₁.subst subsmap) (x₂.subst subsmap)
+  | .getAttr x₁ attr => .getAttr (x₁.subst subsmap) attr
+  | .hasAttr x₁ attr => .hasAttr (x₁.subst subsmap) attr
+  | .set xs => .set (xs.map₁ λ ⟨x, _⟩ => x.subst subsmap)
+  | .record pairs => .record (pairs.attach₂.map λ ⟨(k, v), _⟩ => (k, v.subst subsmap))
+  | .call xfn xs => .call xfn (xs.map₁ λ ⟨x, _⟩ => x.subst subsmap)
+  | .unknown u => match subsmap.find? u with
+    | some val => val.asPartialExpr
+    | none => .unknown u -- no substitution available
+
+/--
+  Given a map of unknown-name to value, substitute all unknowns with the
+  corresponding values, producing a new `Partial.Value`.
+  It's fine for some unknowns to not be in `subsmap`, in which case the returned
+  `Partial.Value` will still contain some unknowns.
+-/
+def Value.subst (subsmap : Map Unknown Partial.Value) : Partial.Value → Partial.Value
+  | .residual r => .residual (r.subst subsmap)
+  | .value v    => .value v -- doesn't contain unknowns, nothing to substitute
 
 end Cedar.Partial
