cedar-lean/Cedar/Data/SizeOf.lean
@@ -1,0 +1,98 @@
+/-
+ Copyright Cedar Contributors
+
+ Licensed under the Apache License, Version 2.0 (the "License");
+ you may not use this file except in compliance with the License.
+ You may obtain a copy of the License at
+
+      https://www.apache.org/licenses/LICENSE-2.0
+
+ Unless required by applicable law or agreed to in writing, software
+ distributed under the License is distributed on an "AS IS" BASIS,
+ WITHOUT WARRANTIES OR CONDITIONS OF ANY KIND, either express or implied.
+ See the License for the specific language governing permissions and
+ limitations under the License.
+-/
+
+import Cedar.Data.Map
+import Cedar.Data.Set
+
+/-!
+  Lemmas involving `sizeOf`, which are located here rather than in `Cedar/Thm`
+  because they are needed for some definitions in `Cedar/Spec` and/or
+  `Cedar/Partial`, and our convention prevents files in `Cedar/Spec` or
+  `Cedar/Partial` from depending on lemmas in `Cedar/Thm`.
+-/
+
+namespace Cedar.Data.Map
+
+/-! ## Map -/
+
+theorem sizeOf_lt_of_value [SizeOf α] [SizeOf β] {m : Map α β} {k : α} {v : β}
+  (h : (k, v) ∈ m.1) :
+  sizeOf v < sizeOf m
+:= by
+  simp only [Membership.mem] at h
+  replace h := List.sizeOf_lt_of_mem h
+  have v_lt_kv : sizeOf v < sizeOf (k, v) := by
+    simp only [sizeOf, Prod._sizeOf_1]
+    omega
+  have m1_lt_m : sizeOf m.1 < sizeOf m := by
+    simp only [sizeOf, Map._sizeOf_1]
+    omega
+  let a := sizeOf v
+  let c := sizeOf m.1
+  let d := sizeOf m
+  have v_lt_m1 : a < c := by apply Nat.lt_trans v_lt_kv h
+  have v_lt_m : a < d := by apply Nat.lt_trans v_lt_m1 m1_lt_m
+  have ha : a = sizeOf v := by simp
+  have hd : d = sizeOf m := by simp
+  rw [ha, hd] at v_lt_m
+  exact v_lt_m
+
+theorem sizeOf_lt_of_kvs [SizeOf α] [SizeOf β] (m : Map α β) :
+  sizeOf m.kvs < sizeOf m
+:= by
+  unfold kvs
+  conv => rhs ; unfold sizeOf _sizeOf_inst _sizeOf_1 ; simp only
+  generalize sizeOf m.1 = s
+  omega
+
+theorem sizeOf_lt_of_tl [SizeOf α] [SizeOf β] {m : Map α β} {tl : List (α × β)}
+  (h : m.kvs = (k, v) :: tl) :
+  1 + sizeOf tl < sizeOf m
+:= by
+  conv => rhs ; unfold sizeOf _sizeOf_inst _sizeOf_1
+  simp only
+  unfold kvs at h
+  simp only [h, List.cons.sizeOf_spec, Prod.mk.sizeOf_spec]
+  generalize sizeOf k = kn
+  generalize sizeOf v = vn
+  generalize sizeOf tl = tn
+  omega
+
+end Cedar.Data.Map
+
+namespace Cedar.Data.Set
+
+/-! ## Set -/
+
+theorem sizeOf_lt_of_mem [SizeOf α] {s : Set α}
+  (h : a ∈ s) :
+  sizeOf a < sizeOf s
+:= by
+  simp only [Membership.mem, elts] at h
+  replace h := List.sizeOf_lt_of_mem h
+  have _ : sizeOf s.1 < sizeOf s := by
+    simp only [sizeOf, _sizeOf_1]
+    omega
+  omega
+
+theorem sizeOf_lt_of_elts [SizeOf α] {s : Set α} :
+  sizeOf s.elts < sizeOf s
+:= by
+  simp only [elts]
+  conv => rhs ; unfold sizeOf _sizeOf_inst _sizeOf_1 ; simp
+  omega
+
+end Cedar.Data.Set
